tests/lean/run/explicitApp.lean
@@ -1,0 +1,27 @@
+/-!
+# Tests for app elaborator in explicit mode
+-/
+
+namespace Test1
+
+/-!
+Named arguments in explicit mode cause arguments it depends on to become implicit.
+However, inst implicit arguments had odd behavior with `_`, since supplying `_` would override
+the fact that it should be implicit.
+-/
+
+theorem foo {p : Prop} [Decidable p] (h : ite p x y = x) : p := sorry
+
+variable {p : Prop} [Decidable p] {α : Type} (x y : α) (h : ite p x y = x)
+
+example : p := @foo (h := h)
+/--
+error: function expected at
+  foo h
+term has type
+  p
+-/
+#guard_msgs in
+example : p := @foo (h := h) _
+
+end Test1
